\documentclass{article}
\usepackage{xeCJK}
\usepackage{amsmath}

\setCJKmainfont{Microsoft YaHei}
\linespread{1.5}

\begin{document}
1.证：\\
下面证明\(f(n) = \sum_{i = 1}^{n}i^{2} = \frac{1}{6}n(n + 1)(2n + 1)\),\\
当\(n = 1\)时, \(f(1) = 1\),\\
假设\(n = k\)时, \(f(n) = \frac{1}{6}n(n + 1)(2n + 1)\)成立,\\
当\(n = k + 1\)时, \[\begin{aligned}
f(n + 1) & = f(n) + (n + 1)^{2} \\
 & = \frac{1}{6}n(n + 1)(2n + 1) + (n + 1)^{2} \\
 & = \frac{1}{6}(n + 1)(n + 1 + 1)\left( 2(n + 1) + 1 \right)
\end{aligned}\] 从而\(f(n) = \frac{1}{6}n(n + 1)(2n + 1)\)

故\(f(n) = \Theta(n^{3})\)

\hfill\break
2.解：\\
(1) \(T(n) = O(n)\)\\
即证\(\exists c,n_{0} > 0,s.t.当n > n_{0},T(n) \leq cn\)\\

假设\(n < k\)时均成立,\\
当\(n = k\)时，\\
\[T(k) = T\left( \frac{k}{2} \right) + k \leq c\frac{k}{2} + k = \left( \frac{c}{2} + 1 \right)k \leq ck,\ c \geq 2,\]
即为\(T(n) = O(n)\)\\
\(T(n) = \Omega(n)\)\\

即证\(\exists c,n_{0} > 0,s.t.当n > n_{0},T(n) \geq cn\)\\
假设\(n < k\)时均成立,\\
当\(n = k\)时，\\
\[T(k) = T\left( \frac{k}{2} \right) + k \geq c\frac{k}{2} + k = \left( \frac{c}{2} + 1 \right)k \geq ck,\ c \leq 2,\]

即为\(T(n) = \Omega(n)\)\\
(2) \(T(n) = O\left( n\log^{2}n \right)\)\\
即证\(\exists c,n_{0} > 0,s.t.当n > n_{0},T(n) \leq cn\log^{2}n\)\\

假设\(n < k\)时均成立,\\
当\(n = k\)时, \[\begin{aligned}
T(k) & = 2T\left( \frac{k}{2} \right) + k\log k \leq c\frac{k}{2}\log^{2}\frac{k}{2} + k\log k \\
 & = ck\log^{2}k + \left( 1 - 2c\log 2 \right)n\log n + cn\log^{2}2 \\
 & \leq ck\log^{2}k,\ c = 1,n_{0} \geq 10,
\end{aligned}\] 即为\(T(n) = O\left( n\log^{2}n \right)\)\\
\(T(n) = \Omega(n\log^{2}n)\)\\

即证\(\exists c,n_{0} > 0,s.t.当n > n_{0},T(n) \geq cn\log^{2}n\)\\
假设\(n < k\)时均成立,\\
当\(n = k\)时, \[\begin{aligned}
T(k) & = 2T\left( \frac{k}{2} \right) + k\log^{2}k \geq c\frac{k}{2}\log^{2}\frac{k}{2} + k\log k \\
 & = ck\log^{2}k + \left( 1 - 2c\log 2 \right)n\log n + cn\log^{2}2 \\
 & \geq ck\log^{2}k,\ c = \frac{1}{2},n_{0} \geq 5,
\end{aligned}\]

即为\(T(n) = \Omega(n\log^{2}n)\)\\
3.证:\\
对于\(\forall x > - 1,x > \ln(x + 1)\),\\
从而 \[\begin{aligned}
1 + \frac{1}{2} + \frac{1}{3} + \ldots + \frac{1}{n} & \geq \ln(\frac{2}{1}) + \ln(\frac{3}{2}) + \ldots + \ln(\frac{n + 1}{n}) \\
 & = \ln(\frac{2}{1} \cdot \frac{3}{2} \cdot \ldots \cdot \frac{n + 1}{n}) \\
 & = \ln(n + 1)
\end{aligned}\]

4.解:\\
\(T(n) = O\left( n^{2} \right)\)\\
即证\(\exists c,n_{0} > 0,s.t.当n > n_{0},T(n) \leq cn^{2}\)\\

假设\(n < k\)时均成立,\\
当\(n = k\)时，\\
\[T(k) = 2T\left( \frac{k}{2} \right) + k^{2} \leq c\left( \frac{k}{2} \right)^{2} + k^{2} = \left( \frac{c}{4} + 1 \right)k^{2} \leq ck^{2},\ c \geq \frac{4}{3},\]
即为\(T(n) = O\left( n^{2} \right)\)\\
\(T(n) = \Omega(n^{2})\)\\

即证\(\exists c,n_{0} > 0,s.t.当n > n_{0},T(n) \geq cn^{2}\)\\
假设\(n < k\)时均成立,\\
当\(n = k\)时，\\
\[T(k) = 2T\left( \frac{k}{2} \right) + k^{2} \geq c\left( \frac{k}{2} \right)^{2} + k^{2} = \left( \frac{c}{4} + 1 \right)k^{2} \geq ck^{2},\ c \leq \frac{4}{3},\]

即为\(T(n) = \Omega(n^{2})\)\\
5.解:\\
\(T(n) = \Omega(n\log n)\)\\

即证\(\exists m,n_{0} > 0,s.t.当n > n_{0},T(n) \geq mn\log n\)\\
假设\(n < k\)时均成立,\\
当\(n = k\)时，\\
\[\begin{aligned}
T(k) & = T\left( \frac{k}{3} \right) + T\left( \frac{2k}{3} \right) + ck \\
 & \geq mc\frac{k}{3}\log\frac{k}{3} + mc\frac{2k}{3}\log\frac{2k}{3} + ck \\
 & = cmk\log k + \left( \frac{2}{3}\log 2 - \log 3 \right)cmk + ck
\end{aligned}\] 当\(c \leq 1\), 取\(m < \frac{1}{3\log 3 - 2\log 2}\),
即有\(T(k) \geq k\log k\),\\
当\(c > 1\), 取\(m > \frac{1}{3\log 3 - 2\log 2},n_{0} = 10\),
即有\(T(k) \geq k\log k\),

即为\(T(n) = \Omega(n\log n)\)\\

\end{document}
