\documentclass{article}
\usepackage{xeCJK}
\usepackage{amsmath}
\usepackage{geometry}


\setCJKmainfont{Microsoft YaHei}
\linespread{1.5}
\setlength{\parindent}{0pt}
\geometry{a4paper,scale=0.75}

\begin{document}
1.\\
设 $P(x)$ 表示 $x$ 是无知的 \\
设 $Q(x)$ 表示 $x$ 是教授 \\
设 $R(x)$ 表示 $x$ 是虚荣的 \\
(1)$\forall x (Q(x) \to \neg P(x))$ \\
(2)$\forall x (P(x) \to R(x))$ \\
(3)$\forall x (Q(x) \to \neg R(x))$ 

2.\\
(1)
\[
\begin{aligned}
&(1)A \to \exists v B, A \vdash A \quad (\in) \\
&(2)A \to \exists v B, A \vdash A \to \exists v B \quad (\in) \\
&(3)A \to \exists v B, A \vdash \exists v B \quad (1)(2)(\to -) \\
&(4)A \to \exists v B, A, B \vdash B \quad (\in) \\
&(5)A \to \exists v B, A \vdash B \quad (3)(4)(\mbox{定理}10) \\
&(6)A \to \exists v B \vdash A \to B \quad (5)(\to +) \\
&(7)\vdash (A \to \exists v B) \to (A \to B) \quad (6)(\to +) \\
&(8)(A \to B) \to \exists v (A \to B) \quad (\mbox{定理}2) \\
&(9)\vdash (A \to \exists v B) \to \exists v (A \to B) \quad (7)(8)(PC\mbox{定理}8)
\end{aligned}    
\]
(2)
\[
\begin{aligned}
&(1)\exists v (A \to B), A \vdash \exists v (A \to B) \quad (\in) \\
&(2)\exists v (A \to B), A, A \to B \vdash A \quad (\in) \\
&(3)\exists v (A \to B), A, A \to B \vdash A \to B \quad (\in) \\
&(4)\exists v (A \to B), A, A \to B \vdash B \quad (2)(3)(\to -) \\
&(5)\exists v (A \to B), A \vdash B \quad (1)(4)(\mbox{定理}10) \\
&(6)B \to \exists v B \quad (\mbox{定理}2) \\
&(7)\exists v (A \to B), A \vdash \exists v B \quad (5)(6)(\to -) \\
&(8)\exists v (A \to B) \vdash A \to \exists v B \quad (7)(\to -) \\
&(9)\vdash \exists v (A \to B) \to (A \to \exists v B) \quad (8)(\to -)
\end{aligned}    
\]
(3)
\[
\begin{aligned}
&(1)\forall v B \to A, B \vdash B \quad (\in) \\
&(2)\forall v B \to A, B \vdash \forall v B \quad (\mbox{定理}4) \\
&(3)\forall v B \to A, B \vdash \forall v B \to A \quad (\in) \\
&(4)\forall v B \to A, B \vdash A \quad (2)(3)(\to -) \\
&(5)\forall v B \to A \vdash B \to A  \quad (4)(\to +) \\
&(6)\vdash (\forall v B \to A) \to (B \to A) \quad (4)(\to +) \\
&(7)(B \to A) \to \exists v (B \to A) \quad (\mbox{定理}2) \\
&(8)\vdash (\forall v B \to A) \to \exists v (B \to A) \quad (6)(7)(PC\mbox{定理}8)
\end{aligned}    
\]
(4)
\[
\begin{aligned}
&(1)\exists v (B \to A), \forall v B \vdash \exists v (B \to A) \quad (\in) \\
&(2)\exists v (B \to A), \forall v B, B \to A \vdash \forall v B \quad (\in) \\
&(3)\exists v (B \to A), \forall v B, B \to A \vdash B \quad (2)(\mbox{定理}1) \\
&(4)\exists v (B \to A), \forall v B, B \to A \vdash B \to A \quad (\in) \\
&(5)\exists v (B \to A), \forall v B, B \to A \vdash A  \quad (3)(4)(\to -) \\
&(6)\exists v (B \to A), \forall v B \vdash A \quad (1)(5)(\mbox{定理}10) \\
&(7)\exists v (B \to A) \vdash \forall v B \to A \quad (6)(\to +) \\
&(8)\vdash \exists v (B \to A) \to (\forall v B \to A) \quad (7)(\to +)
\end{aligned}    
\]
3.\\
(1)
\[
\begin{aligned}
&(1)\forall x (A \to B), A \vdash \forall x (A \to B) \quad (\in) \\
&(2)\forall x (A \to B) \to (\forall x A \to \forall x B) \quad (A_5) \\
&(3)\forall x (A \to B), A \vdash \forall x A \to \forall x B \quad (1)(2)(\to -) \\
&(4)\forall x (A \to B), A \vdash A \quad (\in) \\
&(5)A \to \forall x A \quad (A_6) \\
&(6)\forall x (A \to B), A \vdash \forall x A \quad (4)(5)(\to -) \\
&(7)\forall x (A \to B), A \vdash \forall x B \quad (3)(6)(\to -) \\
&(8)\forall x (A \to B) \vdash (A \to \forall x B) \quad (7)(\to +) \\
&(9)A \to \forall x B, A \vdash A \quad (\in) \\
&(10)A \to \forall x B, A \vdash A \to \forall x B \quad (\in) \\
&(11)A \to \forall x B, A \vdash \forall x B \quad (9)(10)(\to -) \\
&(12)\forall x B \to B \quad (\mbox{定理}1) \\
&(13)A \to \forall x B, A \vdash B \quad (11)(12)(\to -) \\
&(14)A \to \forall x B \vdash A \to B \quad (13)(\to +) \\
&(15)A \to \forall x B \vdash \forall x (A \to B) \quad (14)(\mbox{定理4}) \\
&(16)\forall x (A \to B) \vdash \dashv (A \to \forall x B) \quad (8)(15)(\vdash \dashv  +)
\end{aligned}    
\]
(2)
\[
\begin{aligned}
&(1)\forall x (A \to B), \exists x A \vdash \exists x A \quad (\in) \\
&(2)\forall x (A \to B), \exists x A, A \vdash \forall x (A \to B) \quad (\in) \\
&(3)\forall x (A \to B) \to (A \to B) \quad (\mbox{定理}1) \\
&(4)\forall x (A \to B), \exists x A, A \vdash A \to B \quad (2)(3)(\to -) \\
&(5)\forall x (A \to B), \exists x A, A \vdash A \quad (\in) \\
&(6)\forall x (A \to B), \exists x A, A \vdash B \quad (4)(5)(\to -) \\
&(7)\forall x (A \to B), \exists x A \vdash B \quad (1)(6)(\mbox{定理}10) \\
&(8)\forall x (A \to B) \vdash \exists x A \to B  \quad (7)(\to +) \\
&(9)\exists x A \to B, A \vdash A \quad (\in) \\
&(10)\exists x A \to B, A \vdash \exists x A \quad (9)(\mbox{定理}2) \\
&(11)\exists x A \to B, A \vdash \exists x A \to B \quad (\in) \\
&(12)\exists x A \to B, A \vdash B \quad (10)(11)(\to -) \\
&(13)\exists x A \to B \vdash A \to B \quad (12)(\to +) \\
&(14)\exists x A \to B \vdash \forall x (A \to B) \quad (13)(\mbox{定理}4) \\
&(15)\forall x (A \to B) \vdash \dashv \exists x A \to B \quad (8)(14)(\vdash \dashv  +)
\end{aligned}
\]
(3)
\[
\begin{aligned}
&(1)\forall x (A \wedge B) \vdash \forall x (A \wedge B) \quad (\in) \\
&(2)\forall x (A \wedge B) \to (A \wedge B) \quad (\mbox{定理}1) \\
&(3)\forall x (A \wedge B) \vdash A \wedge B \quad (1)(2)(\to -) \\
&(4)\forall x (A \wedge B) \vdash A \quad (3)(\wedge -) \\
&(5)\forall x (A \wedge B) \vdash B \quad (3)(\wedge -) \\
&(6)\forall x (A \wedge B) \vdash \forall x A \quad (4)(\mbox{定理}5) \\
&(7)\forall x (A \wedge B) \vdash \forall x B \quad (5)(\mbox{定理}5) \\
&(8)\forall x (A \wedge B) \vdash \forall x A \wedge \forall x B \quad (6)(7)(\wedge +) \\
&(9)\forall x A \wedge \forall x B \vdash \forall x A \wedge \forall x B \quad (\in) \\
&(10)\forall x A \wedge \forall x B \vdash \forall x A \quad (9)(\wedge -) \\
&(11)\forall x A \to A \quad (\mbox{定理}1) \\
&(12)\forall x A \wedge \forall x B \vdash A \quad (10)(11)(\to -) \\
&(13)\forall x A \wedge \forall x B \vdash \forall x B \quad (10)(\wedge -) \\
&(14)\forall x B \to B \quad (\mbox{定理}1) \\
&(15)\forall x A \wedge \forall x B \vdash B \quad (13)(14)(\to -) \\
&(16)\forall x A \wedge \forall x B \vdash A \wedge B \quad (12)(15)(\wedge +) \\
&(17)\forall x A \wedge \forall x B \vdash \forall x (A \wedge B) \quad (16)(\mbox{定理}5) \\ 
&(18)\forall x (A \wedge B) \vdash \dashv \forall x A \wedge \forall x B \quad (8)(17)(\vdash \dashv  +)
\end{aligned}    
\]
(4)
\[
\begin{aligned}
&(1)\exists x (A \vee B) \vdash \exists x (A \vee B) \quad (\in) \\
&(2)\exists x (A \vee B), A \vee B \vdash A \vee B \quad (\in) \\
&(3)\exists x (A \vee B), A \vee B, A \vdash A \quad (\in) \\
&(4)\exists x (A \vee B), A \vee B, A \vdash \exists x A \quad (3)(\mbox{定理}2) \\
&(5)\exists x (A \vee B), A \vee B, A \vdash \exists x A \vee \exists x B \quad (4)(\vee +) \\
&(6)\exists x (A \vee B), A \vee B, B \vdash B \quad (\in) \\
&(7)\exists x (A \vee B), A \vee B, B \vdash \exists x B \quad (6)(\mbox{定理}2) \\
&(8)\exists x (A \vee B), A \vee B, B \vdash \exists x A \vee \exists x B \quad (7)(\vee +) \\
&(9)\exists x (A \vee B), A \vee B \vdash \exists x A \vee \exists x B \quad (2)(5)(8)(\vee -) \\
&(10)\exists x (A \vee B) \vdash \exists x A \vee \exists x B \quad (1)(9)(\mbox{定理}10) \\
&(11)\exists x A \vee \exists x B \vdash \exists x A \vee \exists x B \quad (\in) \\
&(12)\exists x A \vee \exists x B, \exists x A \vdash \exists x A \quad (\in) \\
&(13)\exists x A \vee \exists x B, \exists x A, A \vdash A \quad (\in) \\
&(14)\exists x A \vee \exists x B, \exists x A, A \vdash A \vee B \quad (13)(\vee +) \\
&(15)\exists x A \vee \exists x B, \exists x A \vdash A \vee B \quad (12)(14)(\mbox{定理}10)\\
&(16)\exists x A \vee \exists x B, \exists x B \vdash \exists x B \quad (\in) \\
&(17)\exists x A \vee \exists x B, \exists x B, B \vdash B \quad (\in) \\ 
&(18)\exists x A \vee \exists x B, \exists x B, B \vdash A \vee B \quad (17)(\vee +) \\
&(19)\exists x A \vee \exists x B, \exists x B \vdash A \vee B \quad (16)(18)(\mbox{定理}10)\\
&(20)\exists x A \vee \exists x B \vdash A \vee B \quad (11)(15)(19)(\vee -) \\
&(21)\exists x A \vee \exists x B \vdash \exists x (A \vee B) \quad (20)(\mbox{定理}2) \\
&(22)\exists x (A \vee B) \vdash \dashv \exists x A \vee \exists x B \quad (10)(21)(\vdash \dashv  +)
\end{aligned}    
\]
\end{document}