\documentclass{article}
\usepackage{xeCJK}
\usepackage{amsmath}
\usepackage{geometry}


\setCJKmainfont{Microsoft YaHei}
\linespread{1.5}
\setlength{\parindent}{0pt}
\geometry{a4paper,scale=0.75}

\begin{document}
1.\\
(1)
\[
\begin{aligned}
&(1)B \to A \quad \mbox{(假设)}\\
&(2)\neg A \quad \mbox{(假设)} \\
&(3)A \to \neg \neg A \quad \mbox{(定理12)} \\
&(4)B \to \neg \neg A \quad \mbox{((1)(3)定理8)} \\
&(5)\neg \neg B \to B \quad \mbox{(定理10)} \\
&(6)\neg \neg B \to \neg \neg A \quad \mbox{((5)(4)定理8)} \\
&(7)(\neg \neg B \to \neg \neg A) \to (\neg A \to \neg B) \quad \mbox{(公理3)} \\
&(8)\neg A \to \neg B \quad \mbox{((6)(7)rmp分离规则)} \\
&(9)\neg B \quad \mbox{((2)(8)rmp分离规则)} \\
&(10)B \to A,\; \neg A \vdash \neg B \\
&(11)B \to A \vdash (\neg A \to \neg B) \\
&(12)(B \to A) \to (\neg A \to \neg B) \\
\end{aligned}
\]
(2)
\[
\begin{aligned}
&(1)A \to B \quad \mbox{(假设)}\\
&(2)B \to C \quad \mbox{(假设)} \\
&(3)A \quad \mbox{(假设)} \\
&(4)B \quad \mbox{((3)(1)rmp分离规则)} \\
&(5)C \quad \mbox{((4)(2)rmp分离规则)} \\
&(6)A \to B,\; B \to C,\; A \vdash C \\
&(7)A \to B,\; B \to C \vdash A \to C \\
&(8)A \to B \vdash (B \to C) \to (A \to C) \\
&(9)(A \to B) \to ((B \to C) \to (A \to C)) \\
\end{aligned}
\]
(3)
\[
\begin{aligned}
&(1)(A \to B) \to A \quad \mbox{(假设)}\\
&(2)\neg A \to A \quad \mbox{((1)定理18)} \\
&(3)(\neg A \to A) \to A \quad \mbox{(定理9)} \\
&(4)A \quad \mbox{((2)(3)rmp分离规则)} \\
&(5)(A \to B) \to A \vdash A \\
&(6)((A \to B) \to A) \to A \\
\end{aligned}
\]
(4)
\[
\begin{aligned}
&(1)\neg (A \to B) \quad \mbox{(假设)}\\
&(2)B \quad \mbox{(假设)} \\
&(3)\neg A \to (A \to B) \quad \mbox{(定理6)} \\
&(4)(\neg A \to (A \to B)) \to (\neg (A \to B) \to \neg \neg A)\quad \mbox{(定理14)} \\
&(5)\neg (A \to B) \to \neg \neg A \quad \mbox{((3)(4)rmp分离规则)} \\
&(6)\neg \neg A \to A \quad \mbox{(定理10)}\\
&(7)\neg (A \to B) \to A \quad \mbox{((5)(6)定理8)}\\
&(8)A \quad \mbox{((1)(7)rmp分离规则)}\\
&(9)\neg (A \to B),\; B \vdash A\\
&(9)\neg (A \to B) \vdash B \to A \\
&(9)(\neg (A \to B)) \to (B \to A) \\
\end{aligned}
\]
2.\\
(1)
\[
\begin{aligned}
&(1)(\neg A \to \neg B) \to (B \to A) \quad \mbox{(公理3)}\\
&(2)B \to ((\neg A \to \neg B) \to A) \quad \mbox{(定理2)} \\
&(3)A \to ((\neg A \to \neg B) \to A)\quad \mbox{(公理1)} \\
&(4)\neg \neg A \to A \quad \mbox{(定理10)} \\
&(5)\neg \neg A \to ((\neg A \to \neg B) \to A) \quad \mbox{((4)(3)定理8)} \\
&(6)(\neg A \to B) \to ((\neg A \to \neg B) \to A) \quad \mbox{((2)(5)定理18)} \\
\end{aligned}
\]
(2)
\[
\begin{aligned}
&(1)B \to (\neg A \to B) \quad \mbox{(公理1)}\\
&(2)(\neg A \to B) \to ((\neg A \to \neg B) \to A) \quad \mbox{(公理3)} \\
&(3)B \to ((\neg A \to \neg B) \to A) \quad \mbox{((1)(2)定理8)} \\
&(4)(\neg A \to \neg B) \to (B \to A) \quad \mbox{(定理2)} \\
\end{aligned}
\]
\end{document}